Proof of top-level security.

sha3/proof/BlockSponge.ec
@@ -24,7 +24,6 @@ clone import IRO as BIRO with
   op valid  <- valid_block,
   op dto    <- bdistr.
 
-
 (*------ Validity and Parsing/Formatting of Functionality Queries ------*)
 
 op format (p : block list) (n : int) = p ++ nseq (n - 1) b0.
@@ -35,23 +34,15 @@ axiom parseK p n: 0 < n => valid_block p => parse (format p n) = (p,n).
 axiom parse_nil: parse [] = ([],0).
 
 lemma parse_injective: injective parse.
-proof. by move=> bs1 bs2 eq_format; rewrite -formatK eq_format (@formatK bs2). qed.
+proof.
+by move=> bs1 bs2 eq_format; rewrite -formatK eq_format (@formatK bs2).
+qed.
 
 lemma parse_valid p: valid_block p => parse p = (p,1).
 proof.
 move=>h;cut{1}->:p=format p 1;2:smt(parseK).
 by rewrite/format/=nseq0 cats0.
 qed.
-
-
-(*------------------------------ Counter -------------------------------*)
-
-module C = {
-  var c : int
-  proc init() = {
-    c <- 0;
-  }
-}.
 
 (*---------------------------- Restrictions ----------------------------*)
 
@@ -61,33 +52,41 @@ module C = {
     message contains and the number of additional blocks the squeezing
     phase has to output.
   *)
-module FC (F : DFUNCTIONALITY) = {
-  proc init () : unit = {}
-  proc f (bl : block list, nb : int) = {
-    var r : block list <- [];
-    if (0 < nb) {
-      if (C.c + size bl + nb - 1 <= max_size) {
-        C.c <- C.c + size bl + nb - 1;
-        r <@ F.f(bl,nb);
-      }
-    }
-    return r;
+
+module C = {
+  var c : int
+  proc init() = {
+    c <- 0;
   }
 }.
-  
+
+module FC (F : DFUNCTIONALITY) = {
+  proc init () : unit = {}
+
+  proc f (bl : block list, nb : int) = {
+    var z : block list <- [];
+    if (C.c + size bl + (max (nb - 1) 0) <= max_size) {
+      C.c <- C.c + size bl + (max (nb - 1) 0);
+      z <@ F.f(bl, nb);
+    }
+    return z;
+  }
+}.
 
 module PC (P : DPRIMITIVE) = {
   proc init() = {}
+
   proc f (a : state) = {
-    var z : state <- (b0,c0);
+    var z : state <- (b0, c0);
     if (C.c + 1 <= max_size) {
       z <@ P.f(a);
       C.c <- C.c + 1;
     }
     return z;
   }
+
   proc fi (a : state) = {
-    var z : state <- (b0,c0);
+    var z : state <- (b0, c0);
     if (C.c + 1 <= max_size) {
       z <@ P.fi(a);
       C.c <- C.c + 1;
@@ -100,7 +99,7 @@ module DRestr (D : DISTINGUISHER) (F : DFUNCTIONALITY) (P : DPRIMITIVE) = {
   proc distinguish () : bool = {
     var b : bool;
     C.init();
-    b <@ D(FC(F),PC(P)).distinguish();
+    b <@ D(FC(F), PC(P)).distinguish();
     return b;
   }
 }.
@@ -111,13 +110,13 @@ module DRestr (D : DISTINGUISHER) (F : DFUNCTIONALITY) (P : DPRIMITIVE) = {
 module Last (F : DFUNCTIONALITY) : SLCommon.DFUNCTIONALITY = {
   proc init() = {}
   proc f (p : block list) : block = {
-    var r : block list <- [];
-    r <@ F.f(parse p);
-    return last b0 r;
+    var z : block list <- [];
+    z <@ F.f(parse p);
+    return last b0 z;
   }
 }.
 
-module (S : SIMULATOR) (F : DFUNCTIONALITY) = Gconcl.S(Last(F)).
+module (Sim : SIMULATOR) (F : DFUNCTIONALITY) = Gconcl.S(Last(F)).
 
 (*------------------------- Sponge Construction ------------------------*)
 
@@ -155,7 +154,7 @@ module (Sponge : CONSTRUCTION) (P : DPRIMITIVE) : FUNCTIONALITY = {
 lemma conclusion :
     forall (D <: DISTINGUISHER) &m,
       `|  Pr[RealIndif(Sponge, Perm, DRestr(D)).main() @ &m : res]
-        - Pr[IdealIndif(IRO, S, DRestr(D)).main() @ &m : res]|
+        - Pr[IdealIndif(IRO, Sim, DRestr(D)).main() @ &m : res]|
        <= (max_size ^ 2)%r / 2%r * Distr.mu1 dstate witness +
         max_size%r * ((2 * max_size)%r / (2 ^ c)%r) +
         max_size%r * ((2 * max_size)%r / (2 ^ c)%r).
