sha3/proof/SHA3-Security.ec
@@ -1,0 +1,195 @@
+(* Top Level *)
+
+require import AllCore List IntDiv StdOrder Common Sponge. import BIRO.
+require SLCommon BlockSponge.
+
+(* FIX: would be nicer to define limit at top-level and then clone
+   BlockSponge with it - so BlockSponge would then clone lower-level
+   theories with it
+
+op limit : {int | 0 < limit} as gt0_max_limit.
+*)
+
+op limit : int = SLCommon.max_size.
+
+(* FIX: don't want this in bound *)
+
+op dstate : (block * capacity) distr = SLCommon.dstate.
+
+(*---------------------------- Restrictions ----------------------------*)
+
+(** The counter for the functionality counts the number of times the
+    underlying primitive is called inside the functionality. This
+    number is equal to the sum of the number of blocks in the padding
+    of the input, plus the number of additional blocks the squeezing
+    phase has to output.
+  *)
+
+module Cntr = {
+  var c : int
+
+  proc init() = {
+    c <- 0;
+  }
+}.
+
+module FC (F : DFUNCTIONALITY) = {
+  proc init () : unit = {}
+
+  (* ((size bs + 1) %/ r + 1) = size (pad2blocks bs): *)
+
+  proc f (bs : bool list, n : int) : bool list = {
+    var z : bool list <- [];
+    if (Cntr.c +
+        ((size bs + 1) %/ r + 1) +
+        (max ((n + r - 1) %/ r - 1) 0) <= limit) {
+      Cntr.c <-
+        Cntr.c +
+        ((size bs + 1) %/ r + 1) +
+        (max ((n + r - 1) %/ r - 1) 0);
+      z <@ F.f(bs, n);
+    }
+    return z;
+  }
+}.
+
+module PC (P : DPRIMITIVE) = {
+  proc init() = {}
+
+  proc f (a : block * capacity) = {
+    var z : block * capacity <- (b0, c0);
+    if (Cntr.c + 1 <= limit) {
+      z <@ P.f(a);
+      Cntr.c <- Cntr.c + 1;
+    }
+    return z;
+  }
+  proc fi (a : block * capacity) = {
+    var z : block * capacity <- (b0, c0);
+    if (Cntr.c + 1 <= limit) {
+      z <@ P.fi(a);
+      Cntr.c <- Cntr.c + 1;
+    }
+    return z;
+  }
+}.
+
+module DRestr (D : DISTINGUISHER) (F : DFUNCTIONALITY) (P : DPRIMITIVE) = {
+  proc distinguish () : bool = {
+    var b : bool;
+    Cntr.init();
+    b <@ D(FC(F),PC(P)).distinguish();
+    return b;
+  }
+}.
+
+section.
+
+declare module Dist :
+  DISTINGUISHER{Perm, BlockSponge.Sim, IRO, Cntr, BlockSponge.BIRO.IRO,
+                BlockSponge.C}.
+
+lemma drestr_commute1 &m :
+  Pr[BlockSponge.RealIndif
+     (BlockSponge.Sponge, Perm,
+      LowerDist(DRestr(Dist))).main() @ &m : res] =
+  Pr[BlockSponge.RealIndif
+     (BlockSponge.Sponge, Perm,
+      BlockSponge.DRestr(LowerDist(Dist))).main() @ &m : res].
+proof.
+byequiv=> //; proc.
+seq 2 2 : (={glob Dist} /\ ={Perm.m, Perm.mi} ); first sim.
+inline*; wp; sp.
+call (_ : ={c}(Cntr, BlockSponge.C) /\ ={Perm.m, Perm.mi}).
+proc; sp; if=> //; sp; sim.
+proc; sp; if=> //; sp; sim.
+proc=> /=.
+inline BlockSponge.FC(BlockSponge.Sponge(Perm)).f.
+wp; sp.
+if=> //.
+progress; smt(size_pad2blocks).
+seq 1 1 :
+  (={n} /\ nb{2} = (n{2} + r - 1) %/ r /\ bl{2} = pad2blocks bs{1} /\
+   Cntr.c{1} = BlockSponge.C.c{2} /\ ={Perm.m, Perm.mi}).
+auto; progress; by rewrite size_pad2blocks.
+inline RaiseFun(BlockSponge.Sponge(Perm)).f.
+wp; sp.
+call (_ : ={Perm.m, Perm.mi}); first sim.
+auto.
+auto; progress; by rewrite blocks2bits_nil.
+auto.
+qed.
+
+lemma drestr_commute2 &m :
+  Pr[BlockSponge.IdealIndif
+     (BlockSponge.BIRO.IRO, BlockSponge.Sim,
+      LowerDist(DRestr(Dist))).main() @ &m : res] =
+  Pr[BlockSponge.IdealIndif
+     (BlockSponge.BIRO.IRO, BlockSponge.Sim,
+      BlockSponge.DRestr(LowerDist(Dist))).main() @ &m : res].
+proof.
+byequiv=> //; proc.
+seq 2 2 :
+  (={glob Dist, BlockSponge.BIRO.IRO.mp,
+     glob BlockSponge.Sim}); first sim.
+inline*; wp; sp.
+call
+  (_ :
+   ={c}(Cntr, BlockSponge.C) /\ ={BlockSponge.BIRO.IRO.mp} /\
+   ={glob BlockSponge.Sim}).
+proc; sp; if=> //; sim.
+proc; sp; if=> //; sim.
+proc=> /=.
+inline BlockSponge.FC(BlockSponge.BIRO.IRO).f.
+sp; wp.
+if=> //.
+progress; smt(size_pad2blocks).
+seq 1 1 :
+  (={n} /\ nb{2} = (n{2} + r - 1) %/ r /\ bl{2} = pad2blocks bs{1} /\
+   Cntr.c{1} = BlockSponge.C.c{2} /\
+   ={BlockSponge.BIRO.IRO.mp, Gconcl.S.paths, Gconcl.S.mi, Gconcl.S.m}).
+auto; progress.
+rewrite size_pad2blocks //.
+inline RaiseFun(BlockSponge.BIRO.IRO).f.
+wp; sp.
+call (_ : ={BlockSponge.BIRO.IRO.mp}); first sim.
+auto.
+auto; progress; by rewrite blocks2bits_nil.
+auto.
+qed.
+
+lemma security &m :
+  `|Pr[RealIndif(Sponge, Perm, DRestr(Dist)).main() @ &m : res] -
+    Pr[IdealIndif
+       (IRO, RaiseSim(BlockSponge.Sim),
+        DRestr(Dist)).main() @ &m : res]| <=
+  (limit ^ 2)%r / 2%r * Distr.mu1 dstate witness +
+  limit%r * ((2 * limit)%r / (2 ^ c)%r) +
+  limit%r * ((2 * limit)%r / (2 ^ c)%r).
+proof.
+rewrite
+  (RealOrder.ler_trans
+   (`|Pr[BlockSponge.RealIndif
+         (BlockSponge.Sponge, Perm, LowerDist(DRestr(Dist))).main() @ &m : res] -
+      Pr[BlockSponge.IdealIndif
+         (BlockSponge.BIRO.IRO, BlockSponge.Sim,
+          LowerDist(DRestr(Dist))).main() @ &m : res]|))
+  1:RealOrder.lerr_eq
+  1:(conclusion BlockSponge.Sim (DRestr(Dist)) &m) //
+  (drestr_commute1 &m) (drestr_commute2 &m)
+  (BlockSponge.conclusion (LowerDist(Dist)) &m).
+qed.
+
+end section.
+
+lemma SHA3Security
+      (Dist <:
+       DISTINGUISHER{Perm, IRO, BlockSponge.BIRO.IRO, Cntr,
+                     BlockSponge.Sim, BlockSponge.C}) &m :
+  `|Pr[RealIndif(Sponge, Perm, DRestr(Dist)).main() @ &m : res] -
+    Pr[IdealIndif
+       (IRO, RaiseSim(BlockSponge.Sim), DRestr(Dist)).main() @ &m : res]| <=
+    (limit ^ 2)%r / 2%r * (Distr.mu1 dstate witness)%Distr +
+    limit%r * ((2 * limit)%r / (2 ^ c)%r) +
+    limit%r * ((2 * limit)%r / (2 ^ c)%r).
+proof. apply (security Dist &m). qed.
